ulib/FStar.BV.fst
@@ -5,28 +5,49 @@ module B = FStar.BitVector
 
 let bv_t (n : nat) = B.bv_t n
 
-let logand_vec = B.logand_vec
-let logxor_vec = B.logxor_vec
-let logor_vec = B.logor_vec
-let lognot_vec = B.lognot_vec
+let bvand = B.logand_vec
+let bvxor = B.logxor_vec
+let bvor = B.logor_vec
+let bvnot = B.lognot_vec
 
 (*TODO: specify index functions? *)
-let shift_left_vec = B.shift_left_vec
-let shift_right_vec = B.shift_right_vec
+let bvshl = B.shift_left_vec
+let bvshr = B.shift_right_vec
 
-let to_vec = U.to_vec
-let from_vec = U.from_vec
+let int2bv = U.to_vec
+let bv2int = U.from_vec
 
-let to_vec_lemma_1 = U.to_vec_lemma_1
-let to_vec_lemma_2 = U.to_vec_lemma_2
+let int2bv_lemma_1 = U.to_vec_lemma_1
+let int2bv_lemma_2 = U.to_vec_lemma_2
 
-let div_vec #n a b = 
-    U.div_size #n (from_vec #n a) b;
-    to_vec #n (U.div #n (from_vec #n a) b)    
-let mod_vec #n a b = 
-    U.div_size #n (from_vec #n a) b;
-    to_vec #n (U.mod #n (from_vec #n a) b)
-
+let bvdiv #n a b = 
+    int2bv #n (U.udiv #n (bv2int #n a) b)    
+let bvmod #n a b = 
+    int2bv #n (U.mod #n (bv2int #n a) b)
 
 let inverse_vec_lemma = U.inverse_vec_lemma
 let inverse_num_lemma = U.inverse_num_lemma
+
+let int2bv_logand #n #x #y #z pf =
+  inverse_vec_lemma #n (bvand #n (int2bv #n x) (int2bv #n y));
+  ()
+  
+let int2bv_logxor #n #x #y #z pf =
+  inverse_vec_lemma #n (bvxor #n (int2bv x) (int2bv y));
+  ()
+
+let int2bv_logor #n #x #y #z pf =
+  inverse_vec_lemma #n (bvor #n (int2bv x) (int2bv y));
+  ()
+
+let int2bv_shl #n #x #y #z pf =
+  inverse_vec_lemma #n (bvshl #n (int2bv #n x) y);			    
+  ()
+  
+let int2bv_shr #n #x #y #z pf =
+  inverse_vec_lemma #n (bvshr #n (int2bv #n x) y);
+  ()
+
+let int2bv_div #n #x #y #z pf =
+  inverse_vec_lemma #n (bvdiv #n (int2bv #n x) y);
+  ()
