ulib/FStar.Tactics.BV.fst
@@ -3,82 +3,49 @@ module FStar.Tactics.BV
 open FStar.Tactics
 open FStar.Reflection.Syntax
 open FStar.Reflection.Arith
-open FStar.UInt // replace that by some interface
 open FStar.BV
 
-(* Lemmas transforming integer arithmetic to bitvector arithmetic *)
-val to_vec_logand : (#n:pos) -> (#x:uint_t n) -> (#y:uint_t n) -> (#z:bv_t n) ->
-			    squash (logand_vec #n (to_vec #n x) (to_vec #n y) == z) ->
-			    Lemma (to_vec #n (logand #n x y) == z)
-let to_vec_logand #n #x #y #z pf =
-  inverse_vec_lemma #n (logand_vec #n (to_vec x) (to_vec y));
-  ()
-  
-
-val to_vec_logxor : #n:pos -> (#x:uint_t n) -> (#y:uint_t n) -> (#z:bv_t n) ->
-		     squash (logxor_vec (to_vec x) (to_vec y) == z) ->
-		     Lemma (to_vec (logxor x y) == z)
-let to_vec_logxor #n #x #y #z pf =
-  inverse_vec_lemma #n (logxor_vec #n (to_vec x) (to_vec y));
-  ()
-
-val to_vec_logor : #n:pos -> (#x:uint_t n) -> (#y:uint_t n) -> (#z:bv_t n) ->
-		     squash (logor_vec (to_vec x) (to_vec y) == z) ->
-		     Lemma (to_vec (logor x y) == z)
-let to_vec_logor #n #x #y #z pf =
-  inverse_vec_lemma #n (logor_vec #n (to_vec x) (to_vec y));
-  ()
-
-val to_vec_shl : #n:pos -> (#x:uint_t n) -> (#y:uint_t n) -> (#z:bv_t n) ->
-			    squash (shift_left_vec (to_vec x) y == z) ->
-			    Lemma (to_vec (shift_left x y) == z)
-let to_vec_shl #n #x #y #z pf =
-  inverse_vec_lemma #n (shift_left_vec #n (to_vec x) y);			    
-  ()
-  
-val to_vec_shr : #n:pos -> (#x:uint_t n) -> (#y:uint_t n) -> (#z:bv_t n) ->
-			    squash (shift_right_vec (to_vec x) y == z) ->
-			    Lemma (to_vec (shift_right x y) == z)
-let to_vec_shr #n #x #y #z pf =
-  inverse_vec_lemma #n (shift_right_vec #n (to_vec x) y);
-  ()
-
-(* Congruence lemmas used to push integer to bitvector transformations through arguments of expressions *)
-val cong_logand_vec : #n:pos -> (#w:bv_t n) -> (#x:bv_t n) -> 
+(* Congruence lemmas *)
+val cong_bvand : #n:pos -> (#w:bv_t n) -> (#x:bv_t n) -> 
 			       (#y:bv_t n) -> (#z:bv_t n) ->
 			       squash (w == y) -> squash (x == z) ->
-			       Lemma (logand_vec w x == logand_vec y z)
-let cong_logand_vec #n #w #x #y #z pf1 pf2 = ()
+			       Lemma (bvand w x == bvand y z)
+let cong_bvand #n #w #x #y #z pf1 pf2 = ()
 
-val cong_logxor_vec : #n:pos -> (#w:bv_t n) -> (#x:bv_t n) -> 
+val cong_bvxor : #n:pos -> (#w:bv_t n) -> (#x:bv_t n) -> 
 			       (#y:bv_t n) -> (#z:bv_t n) ->
 			       squash (w == y) -> squash (x == z) ->
-			       Lemma (logxor_vec w x == logxor_vec y z)
-let cong_logxor_vec #n #w #x #y #z pf1 pf2 = ()
+			       Lemma (bvxor w x == bvxor y z)
+let cong_bvxor #n #w #x #y #z pf1 pf2 = ()
 
-val cong_logor_vec : #n:pos -> (#w:bv_t n) -> (#x:bv_t n) -> 
+val cong_bvor : #n:pos -> (#w:bv_t n) -> (#x:bv_t n) -> 
 			       (#y:bv_t n) -> (#z:bv_t n) ->
 			       squash (w == y) -> squash (x == z) ->
-			       Lemma (logor_vec w x == logor_vec y z)
-let cong_logor_vec #n #w #x #y #z pf1 pf2 = ()
+			       Lemma (bvor w x == bvor y z)
+let cong_bvor #n #w #x #y #z pf1 pf2 = ()
 
-val cong_shift_left_vec : #n:pos -> (#w:bv_t n) -> (#x:uint_t n) -> 
+val cong_bvshl : #n:pos -> (#w:bv_t n) -> (#x:uint_t' n) -> 
 				 (#y:bv_t n) -> squash (w == y) ->
-				 Lemma (shift_left_vec w x == shift_left_vec y x)
-let cong_shift_left_vec #n #w #x #y pf = ()
+				 Lemma (bvshl w x == bvshl y x)
+let cong_bvshl #n #w #x #y pf = ()
 
-val cong_shift_right_vec : #n:pos -> #w:bv_t #n -> (#x:uint_t n) -> 
-			   #y:bv_t #n -> squash (w == y) ->
-			   Lemma (shift_right_vec w x == shift_right_vec y x)
-let cong_shift_right_vec #n #w #x #y pf = ()
+val cong_bvshr : #n:pos -> #w:bv_t n -> (#x:uint_t' n) -> 
+			   #y:bv_t n -> squash (w == y) ->
+			   Lemma (bvshr #n w x == bvshr #n y x)
+let cong_bvshr #n #w #x #y pf = ()
+
+val cong_bvdiv : #n:pos -> #w:bv_t n -> (#x:uint_t' n{x <> 0}) -> 
+			  #y:bv_t n -> squash (w == y) ->
+			   Lemma (bvdiv #n w x == bvdiv #n y x)
+let cong_bvdiv #n #w #x #y pf = ()
 
 (* Used to reduce the initial equation to an equation on bitvectors*)
-val eq_to_bv: #n:pos -> (#x:uint_t n) -> (#y:uint_t n) ->
-              squash (to_vec #n x == to_vec #n y) -> Lemma (x == y)
-let eq_to_bv #n #x #y pf = to_vec_lemma_2 #n x y
+val eq_to_bv: #n:pos -> (#x:uint_t' n) -> (#y:uint_t' n) ->
+              squash (int2bv #n x == int2bv #n y) -> Lemma (x == y)
+let eq_to_bv #n #x #y pf = int2bv_lemma_2 #n x y
 
-(* Creates two fresh variables and two equations of the form to_vec
-   x = z /\ to_vec y = w. The above lemmas transform these two
+(* Creates two fresh variables and two equations of the form int2bv
+   x = z /\ int2bv y = w. The above lemmas transform these two
    equations before finally instantiating them through reflexivity,
    leaving Z3 to solve z = w *) 
 val trans: #n:pos -> (#x:bv_t n) -> (#y:bv_t n) -> (#z:bv_t n) -> (#w:bv_t n) -> 
@@ -92,27 +59,33 @@ let trans #n #x #y #z #w pf1 pf2 pf3 = ()
  *)
 let rec arith_expr_to_bv e : tactic unit =
     match e with
+    | NatToBv _ (Udiv _ e1 _) | Udiv _ e1 _ ->
+        apply_lemma (quote int2bv_div);;
+        apply_lemma (quote cong_bvdiv);;
+        arith_expr_to_bv e1
     | NatToBv _ (Shl _ e1 _) | Shl _ e1 _ ->
-        apply_lemma (quote to_vec_shl);;
-        apply_lemma (quote cong_shift_left_vec);;
+        apply_lemma (quote int2bv_shl);;
+        apply_lemma (quote cong_bvshl);;
         arith_expr_to_bv e1
     | NatToBv _ (Shr _ e1 _) | Shr _ e1 _ ->
-        apply_lemma (quote to_vec_shr);;
-        apply_lemma (quote cong_shift_right_vec);;
+        apply_lemma (quote int2bv_shr);;
+	dump "after int2bv_Shr";;
+        apply_lemma (quote cong_bvshr);;
+	dump "after cong_bvshr";;
         arith_expr_to_bv e1
     | NatToBv _ (Land _ e1 e2) | (Land _ e1 e2) ->
-        apply_lemma (quote to_vec_logand);;
-        apply_lemma (quote cong_logand_vec);;
+        apply_lemma (quote int2bv_logand);;
+        apply_lemma (quote cong_bvand);;
         arith_expr_to_bv e1;;
         arith_expr_to_bv e2
     | NatToBv _ (Lxor _ e1 e2) | (Lxor _ e1 e2) ->
-        apply_lemma (quote to_vec_logxor);;
-        apply_lemma (quote cong_logxor_vec);;
+        apply_lemma (quote int2bv_logxor);;
+        apply_lemma (quote cong_bvxor);;
         arith_expr_to_bv e1;;
         arith_expr_to_bv e2
     | NatToBv _ (Lor _ e1 e2) | (Lor _ e1 e2) ->
-        apply_lemma (quote to_vec_logor);;
-        apply_lemma (quote cong_logor_vec);;
+        apply_lemma (quote int2bv_logor);;
+        apply_lemma (quote cong_bvor);;
         arith_expr_to_bv e1;;
         arith_expr_to_bv e2	
     | _ ->
@@ -126,8 +99,10 @@ let arith_to_bv_tac : tactic unit =
     | Comp Eq t l r ->
      begin match run_tm (is_arith_expr l) with
       | Inl s ->
+      dump "inl";;
         trefl
       | Inr e ->
+      dump "before seq";;
             seq (arith_expr_to_bv e) trefl
 	   //  arith_expr_to_bv e
         end
@@ -140,6 +115,7 @@ as is for now *)
 let bv_tac ()  =
   apply_lemma (quote eq_to_bv);;
   apply_lemma (quote trans);;
+  dump "after trans";;
   arith_to_bv_tac;;
   arith_to_bv_tac;;
   set_options "--smtencoding.elim_box true";;
